MxDH: separate out generic field components from Montgomery ladder-specific components

src/Examples/ECC/MontgomeryLadder.v
@@ -1,29 +1,37 @@
 Require Import Rupicola.Lib.Api.
+Require Import Rupicola.Examples.ECC.Field.
 Local Open Scope Z_scope.
+
+(* TODO: figure out recursive notation here and move to Notations *)
+Local Notation
+      "'let/d' '''(' x , y ')' := val 'in' body" :=
+  (dlet val
+        (fun v =>
+           let x := fst v in
+           let y := snd v in
+           body))
+    (at level 4, only parsing).
+Local Notation
+      "'let/d' '''(' x , y , z ')' := val 'in' body" :=
+  (dlet val
+        (fun v =>
+           let x := fst (fst v) in
+           let y := snd (fst v) in
+           let z := snd v in
+           body))
+    (at level 4, only parsing).
 
 (* TODO: copy the specs back over into fiat-crypto and prove that they are
    obeyed to validate the slight rephrasings here *)
 Section __.
   Context {semantics : Semantics.parameters}
           {semantics_ok : Semantics.parameters_ok semantics}.
-  Context {mul add sub square scmula24 inv : string}.
-  Context {M a24 : Z}.
-  Context {Finv : Z -> Z}. (* modular inverse in Z/M *)
+  Context {field_parameters : FieldParameters}.
+  Context {bignum_representaton : BignumRepresentation}.
+  Existing Instances spec_of_mul spec_of_square spec_of_add
+           spec_of_sub spec_of_scmula24 spec_of_inv.
 
-  (* In practice, these would be instantiated as:
-     bignum := list word
-     eval := (fun ws => Positional.eval weight n (map word.unsigned ws))
-     Bignum := (fun addr xs =>
-                 (emp (length xs = n) * array scalar addr xs)%sep)
-     bounds := list (option zrange)
-     bounded_by := (fun bs ws =>
-                      list_Z_bounded_by bs (map word.unsigned ws)) *)
-  Context {bignum : Type} {eval : bignum -> Z}
-          {Bignum : word -> bignum -> Semantics.mem -> Prop}
-          {bounds : Type}
-          {bounded_by : bounds -> bignum -> Prop}.
-  Context {loose_bounds tight_bounds : bounds}
-          {relax_bounds :
+  Context {relax_bounds :
              forall X : bignum,
                bounded_by tight_bounds X ->
                bounded_by loose_bounds X}.
@@ -69,25 +77,6 @@ Section __.
     Definition cswap (swap:bool) (a b: point) : point * point :=
       if swap then (b, a) else (a, b).
 
-    (* TODO: figure out recursive notation here and move to Notations *)
-    Local Notation
-          "'let/d' '''(' x , y ')' := val 'in' body" :=
-      (dlet val
-            (fun v =>
-               let x := fst v in
-               let y := snd v in
-               body))
-        (at level 4, only parsing).
-    Local Notation
-          "'let/d' '''(' x , y , z ')' := val 'in' body" :=
-      (dlet val
-            (fun v =>
-               let x := fst (fst v) in
-               let y := snd (fst v) in
-               let z := snd v in
-               body))
-        (at level 4, only parsing).
-
     Definition montladder bound (testbit:nat->bool) (u:Z) : Z :=
       let P1 : point := (1, 0) in
       let P2 : point := (u, 1) in
@@ -110,420 +99,6 @@ Section __.
       let/d r := (x * Finv z) in
       r.
   End Gallina.
-
-  Section Field.
-    Local Notation unop_spec name op xbounds outbounds :=
-      (forall! (x : bignum) (px pout : word) (old_out : bignum),
-          (fun Rr mem =>
-             bounded_by xbounds x
-             /\ (exists Ra, (Bignum px x * Ra)%sep mem)
-             /\ (Bignum pout old_out * Rr)%sep mem)
-            ===> name @ [px; pout] ===>
-            (liftexists out,
-             (emp ((eval out mod M = (op (eval x)) mod M)%Z
-                   /\ bounded_by outbounds out)
-              * Bignum pout out)%sep))
-        (only parsing).
-
-    Local Notation binop_spec name op xbounds ybounds outbounds :=
-      (forall! (x y : bignum) (px py pout : word) (old_out : bignum),
-          (fun Rr mem =>
-             bounded_by xbounds x
-             /\ bounded_by ybounds y
-             /\ (exists Ra, (Bignum px x * Bignum py y * Ra)%sep mem)
-             /\ (Bignum pout old_out * Rr)%sep mem)
-            ===> name @ [px; py; pout] ===>
-            (liftexists out,
-             (emp ((eval out mod M = (op (eval x) (eval y)) mod M)%Z
-                   /\ bounded_by outbounds out)
-              * Bignum pout out)%sep)) (only parsing).
-
-    Instance spec_of_mul : spec_of mul :=
-      binop_spec mul Z.mul loose_bounds loose_bounds tight_bounds.
-    Instance spec_of_square : spec_of square :=
-      unop_spec square (fun x => Z.mul x x) loose_bounds tight_bounds.
-    Instance spec_of_add : spec_of add :=
-      binop_spec add Z.add tight_bounds tight_bounds loose_bounds.
-    Instance spec_of_sub : spec_of sub :=
-      binop_spec sub Z.sub tight_bounds tight_bounds loose_bounds.
-    Instance spec_of_scmula24 : spec_of scmula24 :=
-      unop_spec scmula24 (Z.mul a24) loose_bounds tight_bounds.
-
-    (* TODO: what are the bounds for inv? *)
-    Instance spec_of_inv : spec_of inv :=
-      unop_spec inv Finv tight_bounds loose_bounds.
-  End Field.
-  Existing Instances spec_of_mul spec_of_square spec_of_add
-           spec_of_sub spec_of_scmula24 spec_of_inv.
-
-  Section Compile.
-    (* In compilation, we need to decide where to store outputs. In particular,
-       we don't want to overwrite a variable that we want to use later with the
-       output of some operation. The [Placeholder] alias explicitly signifies
-       which Bignums are overwritable.
-
-       TODO: in the future, it would be nice to be able to look through the
-       Gallina code and see which Bignums get used later and which don't. *)
-    Definition Placeholder := Bignum.
-
-    Lemma compile_mul :
-      forall (locals: Semantics.locals) (mem: Semantics.mem)
-        tr R Rin Rout functions T (pred: T -> _ -> Prop)
-        (x y out : bignum) x_ptr x_var y_ptr y_var out_ptr out_var
-        k k_impl,
-        spec_of_mul functions ->
-        bounded_by loose_bounds x ->
-        bounded_by loose_bounds y ->
-        (Bignum x_ptr x * Bignum y_ptr y * Rin)%sep mem ->
-        (Placeholder out_ptr out * Rout)%sep mem ->
-        map.get locals x_var = Some x_ptr ->
-        map.get locals y_var = Some y_ptr ->
-        map.get locals out_var = Some out_ptr ->
-        let v := (eval x * eval y) mod M in
-        (let head := v in
-         forall out m,
-           eval out mod M = head ->
-           bounded_by tight_bounds out ->
-           sep (Bignum out_ptr out) Rout m ->
-           (find k_impl
-            implementing (pred (k (eval out mod M)))
-            with-locals locals and-memory m and-trace tr and-rest R
-            and-functions functions)) ->
-        (let head := v in
-         find (cmd.seq
-                 (cmd.call [] mul [expr.var x_var; expr.var y_var;
-                                     expr.var out_var])
-                 k_impl)
-         implementing (pred (dlet head k))
-         with-locals locals and-memory mem and-trace tr and-rest R
-         and-functions functions).
-    Proof.
-      cbv [Placeholder] in *.
-      repeat straightline'.
-      handle_call; [ solve [eauto] .. | ].
-      sepsimpl.
-      repeat match goal with x := _ mod M |- _ =>
-                                  subst x end.
-      match goal with H : _ mod M = ?x mod M
-                      |- context [dlet (?x mod M)] =>
-                      rewrite <-H
-      end.
-      eauto.
-    Qed.
-
-    Lemma compile_add :
-      forall (locals: Semantics.locals) (mem: Semantics.mem)
-        tr R Rin Rout functions T (pred: T -> _ -> Prop)
-        (x y out : bignum) x_ptr x_var y_ptr y_var out_ptr out_var
-        k k_impl,
-        spec_of_add functions ->
-        bounded_by tight_bounds x ->
-        bounded_by tight_bounds y ->
-        (Bignum x_ptr x * Bignum y_ptr y * Rin)%sep mem ->
-        (Placeholder out_ptr out * Rout)%sep mem ->
-        map.get locals x_var = Some x_ptr ->
-        map.get locals y_var = Some y_ptr ->
-        map.get locals out_var = Some out_ptr ->
-        let v := (eval x + eval y) mod M in
-        (let head := v in
-         forall out m,
-           eval out mod M = head ->
-           bounded_by loose_bounds out ->
-           sep (Bignum out_ptr out) Rout m ->
-           (find k_impl
-            implementing (pred (k (eval out mod M)))
-            with-locals locals and-memory m and-trace tr and-rest R
-            and-functions functions)) ->
-        (let head := v in
-         find (cmd.seq
-                 (cmd.call [] add [expr.var x_var; expr.var y_var;
-                                     expr.var out_var])
-                 k_impl)
-         implementing (pred (dlet head k))
-         with-locals locals and-memory mem and-trace tr and-rest R
-         and-functions functions).
-    Proof.
-      cbv [Placeholder] in *.
-      repeat straightline'.
-      handle_call; [ solve [eauto] .. | ].
-      sepsimpl.
-      repeat match goal with x := _ mod M |- _ =>
-                                  subst x end.
-      match goal with H : _ mod M = ?x mod M
-                      |- context [dlet (?x mod M)] =>
-                      rewrite <-H
-      end.
-      eauto.
-    Qed.
-
-    Lemma compile_sub :
-      forall (locals: Semantics.locals) (mem: Semantics.mem)
-        tr R Rin Rout functions T (pred: T -> _ -> Prop)
-        (x y out : bignum) x_ptr x_var y_ptr y_var out_ptr out_var
-        k k_impl,
-        spec_of_sub functions ->
-        bounded_by tight_bounds x ->
-        bounded_by tight_bounds y ->
-        (Bignum x_ptr x * Bignum y_ptr y * Rin)%sep mem ->
-        (Placeholder out_ptr out * Rout)%sep mem ->
-        map.get locals x_var = Some x_ptr ->
-        map.get locals y_var = Some y_ptr ->
-        map.get locals out_var = Some out_ptr ->
-        let v := (eval x - eval y) mod M in
-        (let head := v in
-         forall out m,
-           eval out mod M = head ->
-           bounded_by loose_bounds out ->
-           sep (Bignum out_ptr out) Rout m ->
-           (find k_impl
-            implementing (pred (k (eval out mod M)))
-            with-locals locals and-memory m and-trace tr and-rest R
-            and-functions functions)) ->
-        (let head := v in
-         find (cmd.seq
-                 (cmd.call [] sub [expr.var x_var; expr.var y_var;
-                                     expr.var out_var])
-                 k_impl)
-         implementing (pred (dlet head k))
-         with-locals locals and-memory mem and-trace tr and-rest R
-         and-functions functions).
-    Proof.
-      cbv [Placeholder] in *.
-      repeat straightline'.
-      handle_call; [ solve [eauto] .. | ].
-      sepsimpl.
-      repeat match goal with x := _ mod M |- _ =>
-                                  subst x end.
-      match goal with H : _ mod M = ?x mod M
-                      |- context [dlet (?x mod M)] =>
-                      rewrite <-H
-      end.
-      eauto.
-    Qed.
-
-    Lemma compile_square :
-      forall (locals: Semantics.locals) (mem: Semantics.mem)
-        tr R Rin Rout functions T (pred: T -> _ -> Prop)
-        (x out : bignum) x_ptr x_var out_ptr out_var k k_impl,
-        spec_of_square functions ->
-        bounded_by loose_bounds x ->
-        (Bignum x_ptr x * Rin)%sep mem ->
-        (Placeholder out_ptr out * Rout)%sep mem ->
-        map.get locals x_var = Some x_ptr ->
-        map.get locals out_var = Some out_ptr ->
-        let v := (eval x ^ 2) mod M in
-        (let head := v in
-         forall out m,
-           eval out mod M = head ->
-           bounded_by tight_bounds out ->
-           sep (Bignum out_ptr out) Rout m ->
-           (find k_impl
-            implementing (pred (k (eval out mod M)))
-            with-locals locals and-memory m and-trace tr and-rest R
-            and-functions functions)) ->
-        (let head := v in
-         find (cmd.seq
-                 (cmd.call [] square [expr.var x_var; expr.var out_var])
-                 k_impl)
-         implementing (pred (dlet head k))
-         with-locals locals and-memory mem and-trace tr and-rest R
-         and-functions functions).
-    Proof.
-      cbv [Placeholder] in *.
-      repeat straightline'.
-      handle_call; [ solve [eauto] .. | ].
-      sepsimpl.
-      repeat match goal with x := _ mod M |- _ =>
-                                  subst x end.
-      rewrite Z.pow_2_r in *.
-      match goal with H : _ mod M = ?x mod M
-                      |- context [dlet (?x mod M)] =>
-                      rewrite <-H
-      end.
-      eauto.
-    Qed.
-
-    Lemma compile_scmula24 :
-      forall (locals: Semantics.locals) (mem: Semantics.mem)
-        tr R Rin Rout functions T (pred: T -> _ -> Prop)
-        (x out : bignum) x_ptr x_var out_ptr out_var k k_impl,
-        spec_of_scmula24 functions ->
-        bounded_by loose_bounds x ->
-        (Bignum x_ptr x * Rin)%sep mem ->
-        (Placeholder out_ptr out * Rout)%sep mem ->
-        map.get locals x_var = Some x_ptr ->
-        map.get locals out_var = Some out_ptr ->
-        let v := (a24 * eval x) mod M in
-        (let head := v in
-         forall out m,
-           eval out mod M = head ->
-           bounded_by tight_bounds out ->
-           sep (Bignum out_ptr out) Rout m ->
-           (find k_impl
-            implementing (pred (k (eval out mod M)))
-            with-locals locals and-memory m and-trace tr and-rest R
-            and-functions functions)) ->
-        (let head := v in
-         find (cmd.seq
-                 (cmd.call [] scmula24 [expr.var x_var; expr.var out_var])
-                 k_impl)
-         implementing (pred (dlet head k))
-         with-locals locals and-memory mem and-trace tr and-rest R
-         and-functions functions).
-    Proof.
-      cbv [Placeholder] in *.
-      repeat straightline'.
-      handle_call; [ solve [eauto] .. | ].
-      sepsimpl.
-      repeat match goal with x := _ mod M |- _ =>
-                                  subst x end.
-      match goal with H : _ mod M = ?x mod M
-                      |- context [dlet (?x mod M)] =>
-                      rewrite <-H
-      end.
-      eauto.
-    Qed.
-
-    (* noop indicating that the last argument should store output *)
-    Definition overwrite1 {A B} := @id (A -> B).
-    (* noop indicating that the 2nd-to-last argument should store output *)
-    Definition overwrite2 {A B C} := @id (A -> B -> C).
-
-    Lemma compile_compose_l :
-      forall (locals: Semantics.locals) (mem: Semantics.mem)
-        tr R Rout functions T (pred: T -> _ -> Prop)
-        (op1 op2 : Z -> Z -> Z)
-        x y z out out_ptr out_var k k_impl,
-        (Placeholder out_ptr out * Rout)%sep mem ->
-        map.get locals out_var = Some out_ptr ->
-        let v := ((op2 (op1 x y mod M) z)) mod M in
-        (let head := v in
-         (find k_impl
-          implementing (pred (dlet (op1 x y mod M)
-          (fun xy => dlet ((overwrite2 op2) xy z mod M) k)))
-          with-locals locals and-memory mem and-trace tr and-rest R
-          and-functions functions)) ->
-        (let head := v in
-         find k_impl
-         implementing (pred (dlet head k))
-         with-locals locals and-memory mem and-trace tr and-rest R
-         and-functions functions).
-    Proof.
-      cbv [Placeholder overwrite1 overwrite2] in *.
-      repeat straightline'. auto.
-    Qed.
-
-    Lemma compile_compose_r :
-      forall (locals: Semantics.locals) (mem: Semantics.mem)
-        tr R Rout functions T (pred: T -> _ -> Prop)
-        (op1 op2 : Z -> Z -> Z)
-        x y z out out_ptr out_var k k_impl,
-        (Placeholder out_ptr out * Rout)%sep mem ->
-        map.get locals out_var = Some out_ptr ->
-        let v := ((op2 z (op1 x y mod M))) mod M in
-        (let head := v in
-         (find k_impl
-          implementing (pred (dlet (op1 x y mod M)
-          (fun xy => dlet ((overwrite1 op2) z xy mod M) k)))
-          with-locals locals and-memory mem and-trace tr and-rest R
-          and-functions functions)) ->
-        (let head := v in
-         find k_impl
-         implementing (pred (dlet head k))
-         with-locals locals and-memory mem and-trace tr and-rest R
-         and-functions functions).
-    Proof.
-      cbv [Placeholder overwrite1 overwrite2] in *.
-      repeat straightline'. auto.
-    Qed.
-
-    Lemma compile_overwrite1 :
-      forall (locals: Semantics.locals) (mem: Semantics.mem)
-        tr R Rin functions T (pred: T -> _ -> Prop)
-        (x : Z) (op : Z -> Z -> Z) (y : bignum) y_ptr y_var k k_impl,
-        (Bignum y_ptr y * Rin)%sep mem ->
-        map.get locals y_var = Some y_ptr ->
-        let v := ((overwrite1 op) x (eval y mod M)) mod M in
-        let v' := (op x (eval y mod M)) mod M in
-        (let __ := 0 in (* placeholder *)
-         forall m,
-           sep (Placeholder y_ptr y) Rin m ->
-           (find k_impl
-            implementing (pred (dlet v' k))
-            with-locals locals and-memory m and-trace tr and-rest R
-            and-functions functions)) ->
-        (let head := v in
-         find k_impl
-         implementing (pred (dlet head k))
-         with-locals locals and-memory mem and-trace tr and-rest R
-         and-functions functions).
-    Proof.
-      cbv [Placeholder] in *.
-      repeat straightline'. auto.
-    Qed.
-
-    Lemma compile_overwrite2 :
-      forall (locals: Semantics.locals) (mem: Semantics.mem)
-        tr R Rin functions T (pred: T -> _ -> Prop)
-        (y : Z) (op : Z -> Z -> Z) (x : bignum) x_ptr x_var k k_impl,
-        (Bignum x_ptr x * Rin)%sep mem ->
-        map.get locals x_var = Some x_ptr ->
-        let v := ((overwrite2 op) (eval x mod M) y) mod M in
-        let v' := (op (eval x mod M) y) mod M in
-        (let __ := 0 in (* placeholder *)
-         forall m,
-           sep (Placeholder x_ptr x) Rin m ->
-           (find k_impl
-            implementing (pred (dlet v' k))
-            with-locals locals and-memory m and-trace tr and-rest R
-            and-functions functions)) ->
-        (let head := v in
-         find k_impl
-         implementing (pred (dlet head k))
-         with-locals locals and-memory mem and-trace tr and-rest R
-         and-functions functions).
-    Proof.
-      cbv [Placeholder] in *.
-      repeat straightline'. auto.
-    Qed.
-  End Compile.
-
-  (* helper for Zpow_mod *)
-  Lemma Zpow_mod_nonneg a b m :
-    0 <= b -> (a ^ b) mod m = ((a mod m) ^ b) mod m.
-  Proof.
-    intros. revert a m.
-    apply natlike_ind with (x:=b); intros;
-      repeat first [ rewrite Z.pow_0_r
-                   | rewrite Z.pow_succ_r by auto
-                   | reflexivity
-                   | solve [auto] ]; [ ].
-    Z.push_mod.
-    match goal with
-      H : context [ (_ ^ _) mod _ = (_ ^ _) mod _ ] |- _ =>
-      rewrite H end.
-    Z.push_pull_mod. reflexivity.
-  Qed.
-
-  (* TODO: upstream to coqutil's Z.pull_mod *)
-  Lemma Zpow_mod a b m : (a ^ b) mod m = ((a mod m) ^ b) mod m.
-  Proof.
-    destruct (Z_le_dec 0 b); auto using Zpow_mod_nonneg; [ ].
-    rewrite !Z.pow_neg_r by lia. reflexivity.
-  Qed.
-
-  (* TODO: replace with Z.pull_mod once Zpow_mod is upstreamed *)
-  Local Ltac pull_mod :=
-    repeat first [ progress Z.pull_mod
-                 | rewrite <-Zpow_mod ].
-
-  Ltac field_compile_step :=
-    Z.push_pull_mod; pull_mod;
-    first [ simple eapply compile_mul
-          | simple eapply compile_add
-          | simple eapply compile_sub
-          | simple eapply compile_square
-          | simple eapply compile_scmula24 ].
 
   (* single predicate for all ladderstep end-state information *)
   (* N.B. it's important to leave the associativity of the predicate so that the
@@ -579,47 +154,11 @@ Section __.
            (ladderstep_gallina
               (eval X1) (eval X2, eval Z2) (eval X3, eval Z3))).
 
-  Ltac compile_compose_step :=
-    Z.push_mod;
-    first [ simple eapply compile_compose_l
-          | simple eapply compile_compose_r
-          | simple eapply compile_overwrite1
-          | simple eapply compile_overwrite2 ];
-    [ solve [repeat compile_step] .. | intros ].
-
-  Ltac compile_custom ::=
-    repeat compile_compose_step;
-    field_compile_step; [ repeat compile_step .. | ];
-    (* if the output we selected was one of the inputs, need to write the
-       Placeholder back into a Bignum for the arguments precondition *)
-    lazymatch goal with
-    | |- sep _ _ _ =>
-      change Placeholder with Bignum in * |- ;
-      solve [repeat compile_step]
-    | _ => idtac
-    end;
-    [ solve [repeat compile_step] .. | intros ].
-
-  (* only apply compile_step when repeat_compile_step solves all the side
-     conditions but one *)
-  Local Ltac safe_compile_step :=
-    compile_step; [ solve [repeat compile_step] .. | ].
-
-  Ltac lookup_Bignum_pointer x :=
-    lazymatch goal with
-    | H : sep _ _ ?m |- context [?m] =>
-      lazymatch type of H with
-        context [Bignum ?p x] => p
-      end
-    end.
-
-  Local Ltac overwrite p := change (Bignum p) with (Placeholder p) in *.
-
   Derive ladderstep_body SuchThat
          (let args := ["X1"; "X2"; "Z2"; "X3"; "Z3";
-                          "A"; "AA"; "B"; "BB"; "E"; "C";
-                            "D"; "DA"; "CB"] in
-           let ladderstep := ("ladderstep", (args, [], ladderstep_body)) in
+                         "A"; "AA"; "B"; "BB"; "E"; "C";
+                           "D"; "DA"; "CB"] in
+          let ladderstep := ("ladderstep", (args, [], ladderstep_body)) in
           program_logic_goal_for
             ladderstep
             (ltac:(let x := program_logic_goal_for_function
@@ -633,10 +172,10 @@ Section __.
 
     (* by now, we're out of Placeholders; need to decide (manually for now)
        where output gets stored *)
-    overwrite pX3; repeat safe_compile_step.
-    overwrite pZ3; repeat safe_compile_step.
-    overwrite pX2; repeat safe_compile_step.
-    overwrite pZ2; repeat safe_compile_step.
+    overwrite_bignum pX3; repeat safe_compile_step.
+    overwrite_bignum pZ3; repeat safe_compile_step.
+    overwrite_bignum pX2; repeat safe_compile_step.
+    overwrite_bignum pZ2; repeat safe_compile_step.
 
     (* done! now just prove postcondition *)
     compile_done. cbv [LadderStepResult].
