src/Examples/ECC/Field.v
@@ -1,0 +1,484 @@
+Require Import Rupicola.Lib.Api.
+Local Open Scope Z_scope.
+
+Class FieldParameters :=
+  { (** mathematical parameters **)
+    M : Z; (* modulus *)
+    a24 : Z; (* (a+2) / 4 or (a-2) / 4, depending on the implementation *)
+    Finv : Z -> Z; (* modular inverse in Z/M *)
+    (** function names **)
+    mul : string; add : string; sub : string;
+    square : string; scmula24 : string; inv : string;
+  }.
+
+(* In practice, these would be instantiated with:
+   bignum := list word
+   eval := fun ws => Positional.eval weight n (map word.unsigned ws)
+   Bignum := (fun addr xs =>
+               (emp (length xs = n) * array scalar addr xs)%sep)
+   bounds := list (option zrange)
+   bounded_by := (fun bs ws =>
+                   list_Z_bounded_by bs (map word.unsigned ws)) *)
+Class BignumRepresentation :=
+  { bignum : Type;
+    eval : bignum -> Z;
+    Bignum :
+      forall {semantics : Semantics.parameters},
+        word -> bignum -> Semantics.mem -> Prop;
+    bounds : Type;
+    bounded_by : bounds -> bignum -> Prop;
+
+    (* TODO: does this cover all field operation schemes, more than just
+     UnsaturatedSolinas? *)
+    loose_bounds : bounds;
+    tight_bounds : bounds;
+  }.
+
+Section Specs.
+  Context {semantics : Semantics.parameters}
+          {semantics_ok : Semantics.parameters_ok semantics}.
+  Context {field_parameters : FieldParameters}.
+  Context {bignum_representaton : BignumRepresentation}.
+
+  Local Notation unop_spec name op xbounds outbounds :=
+    (forall! (x : bignum) (px pout : word) (old_out : bignum),
+        (fun Rr mem =>
+           bounded_by xbounds x
+           /\ (exists Ra, (Bignum px x * Ra)%sep mem)
+           /\ (Bignum pout old_out * Rr)%sep mem)
+          ===> name @ [px; pout] ===>
+          (liftexists out,
+           (emp ((eval out mod M = (op (eval x)) mod M)%Z
+                 /\ bounded_by outbounds out)
+            * Bignum pout out)%sep))
+      (only parsing).
+
+  Local Notation binop_spec name op xbounds ybounds outbounds :=
+    (forall! (x y : bignum) (px py pout : word) (old_out : bignum),
+        (fun Rr mem =>
+           bounded_by xbounds x
+           /\ bounded_by ybounds y
+           /\ (exists Ra, (Bignum px x * Bignum py y * Ra)%sep mem)
+           /\ (Bignum pout old_out * Rr)%sep mem)
+          ===> name @ [px; py; pout] ===>
+          (liftexists out,
+           (emp ((eval out mod M = (op (eval x) (eval y)) mod M)%Z
+                 /\ bounded_by outbounds out)
+            * Bignum pout out)%sep)) (only parsing).
+
+  Instance spec_of_mul : spec_of mul :=
+    binop_spec mul Z.mul loose_bounds loose_bounds tight_bounds.
+  Instance spec_of_square : spec_of square :=
+    unop_spec square (fun x => Z.mul x x) loose_bounds tight_bounds.
+  Instance spec_of_add : spec_of add :=
+    binop_spec add Z.add tight_bounds tight_bounds loose_bounds.
+  Instance spec_of_sub : spec_of sub :=
+    binop_spec sub Z.sub tight_bounds tight_bounds loose_bounds.
+  Instance spec_of_scmula24 : spec_of scmula24 :=
+    unop_spec scmula24 (Z.mul a24) loose_bounds tight_bounds.
+
+  (* TODO: what are the bounds for inv? *)
+  Instance spec_of_inv : spec_of inv :=
+    unop_spec inv Finv tight_bounds loose_bounds.
+End Specs.
+Existing Instances spec_of_mul spec_of_square spec_of_add
+         spec_of_sub spec_of_scmula24 spec_of_inv.
+
+Section Compile.
+  Context {semantics : Semantics.parameters}
+          {semantics_ok : Semantics.parameters_ok semantics}.
+  Context {field_parameters : FieldParameters}.
+  Context {bignum_representaton : BignumRepresentation}.
+
+  (* In compilation, we need to decide where to store outputs. In particular,
+     we don't want to overwrite a variable that we want to use later with the
+     output of some operation. The [Placeholder] alias explicitly signifies
+     which Bignums are overwritable.
+
+     TODO: in the future, it would be nice to be able to look through the
+     Gallina code and see which Bignums get used later and which don't. *)
+  Definition Placeholder := Bignum.
+
+  Lemma compile_mul :
+    forall (locals: Semantics.locals) (mem: Semantics.mem)
+      tr R Rin Rout functions T (pred: T -> _ -> Prop)
+      (x y out : bignum) x_ptr x_var y_ptr y_var out_ptr out_var
+      k k_impl,
+      spec_of_mul functions ->
+      bounded_by loose_bounds x ->
+      bounded_by loose_bounds y ->
+      (Bignum x_ptr x * Bignum y_ptr y * Rin)%sep mem ->
+      (Placeholder out_ptr out * Rout)%sep mem ->
+      map.get locals x_var = Some x_ptr ->
+      map.get locals y_var = Some y_ptr ->
+      map.get locals out_var = Some out_ptr ->
+      let v := (eval x * eval y) mod M in
+      (let head := v in
+       forall out m,
+         eval out mod M = head ->
+         bounded_by tight_bounds out ->
+         sep (Bignum out_ptr out) Rout m ->
+         (find k_impl
+          implementing (pred (k (eval out mod M)))
+          with-locals locals and-memory m and-trace tr and-rest R
+          and-functions functions)) ->
+      (let head := v in
+       find (cmd.seq
+               (cmd.call [] mul [expr.var x_var; expr.var y_var;
+                                   expr.var out_var])
+               k_impl)
+       implementing (pred (dlet head k))
+       with-locals locals and-memory mem and-trace tr and-rest R
+       and-functions functions).
+  Proof.
+    cbv [Placeholder] in *.
+    repeat straightline'.
+    handle_call; [ solve [eauto] .. | ].
+    sepsimpl.
+    repeat match goal with x := _ mod M |- _ =>
+                                subst x end.
+    match goal with H : _ mod M = ?x mod M
+                    |- context [dlet (?x mod M)] =>
+                    rewrite <-H
+    end.
+    eauto.
+  Qed.
+
+  Lemma compile_add :
+    forall (locals: Semantics.locals) (mem: Semantics.mem)
+      tr R Rin Rout functions T (pred: T -> _ -> Prop)
+      (x y out : bignum) x_ptr x_var y_ptr y_var out_ptr out_var
+      k k_impl,
+      spec_of_add functions ->
+      bounded_by tight_bounds x ->
+      bounded_by tight_bounds y ->
+      (Bignum x_ptr x * Bignum y_ptr y * Rin)%sep mem ->
+      (Placeholder out_ptr out * Rout)%sep mem ->
+      map.get locals x_var = Some x_ptr ->
+      map.get locals y_var = Some y_ptr ->
+      map.get locals out_var = Some out_ptr ->
+      let v := (eval x + eval y) mod M in
+      (let head := v in
+       forall out m,
+         eval out mod M = head ->
+         bounded_by loose_bounds out ->
+         sep (Bignum out_ptr out) Rout m ->
+         (find k_impl
+          implementing (pred (k (eval out mod M)))
+          with-locals locals and-memory m and-trace tr and-rest R
+          and-functions functions)) ->
+      (let head := v in
+       find (cmd.seq
+               (cmd.call [] add [expr.var x_var; expr.var y_var;
+                                   expr.var out_var])
+               k_impl)
+       implementing (pred (dlet head k))
+       with-locals locals and-memory mem and-trace tr and-rest R
+       and-functions functions).
+  Proof.
+    cbv [Placeholder] in *.
+    repeat straightline'.
+    handle_call; [ solve [eauto] .. | ].
+    sepsimpl.
+    repeat match goal with x := _ mod M |- _ =>
+                                subst x end.
+    match goal with H : _ mod M = ?x mod M
+                    |- context [dlet (?x mod M)] =>
+                    rewrite <-H
+    end.
+    eauto.
+  Qed.
+
+  Lemma compile_sub :
+    forall (locals: Semantics.locals) (mem: Semantics.mem)
+      tr R Rin Rout functions T (pred: T -> _ -> Prop)
+      (x y out : bignum) x_ptr x_var y_ptr y_var out_ptr out_var
+      k k_impl,
+      spec_of_sub functions ->
+      bounded_by tight_bounds x ->
+      bounded_by tight_bounds y ->
+      (Bignum x_ptr x * Bignum y_ptr y * Rin)%sep mem ->
+      (Placeholder out_ptr out * Rout)%sep mem ->
+      map.get locals x_var = Some x_ptr ->
+      map.get locals y_var = Some y_ptr ->
+      map.get locals out_var = Some out_ptr ->
+      let v := (eval x - eval y) mod M in
+      (let head := v in
+       forall out m,
+         eval out mod M = head ->
+         bounded_by loose_bounds out ->
+         sep (Bignum out_ptr out) Rout m ->
+         (find k_impl
+          implementing (pred (k (eval out mod M)))
+          with-locals locals and-memory m and-trace tr and-rest R
+          and-functions functions)) ->
+      (let head := v in
+       find (cmd.seq
+               (cmd.call [] sub [expr.var x_var; expr.var y_var;
+                                   expr.var out_var])
+               k_impl)
+       implementing (pred (dlet head k))
+       with-locals locals and-memory mem and-trace tr and-rest R
+       and-functions functions).
+  Proof.
+    cbv [Placeholder] in *.
+    repeat straightline'.
+    handle_call; [ solve [eauto] .. | ].
+    sepsimpl.
+    repeat match goal with x := _ mod M |- _ =>
+                                subst x end.
+    match goal with H : _ mod M = ?x mod M
+                    |- context [dlet (?x mod M)] =>
+                    rewrite <-H
+    end.
+    eauto.
+  Qed.
+
+  Lemma compile_square :
+    forall (locals: Semantics.locals) (mem: Semantics.mem)
+      tr R Rin Rout functions T (pred: T -> _ -> Prop)
+      (x out : bignum) x_ptr x_var out_ptr out_var k k_impl,
+      spec_of_square functions ->
+      bounded_by loose_bounds x ->
+      (Bignum x_ptr x * Rin)%sep mem ->
+      (Placeholder out_ptr out * Rout)%sep mem ->
+      map.get locals x_var = Some x_ptr ->
+      map.get locals out_var = Some out_ptr ->
+      let v := (eval x ^ 2) mod M in
+      (let head := v in
+       forall out m,
+         eval out mod M = head ->
+         bounded_by tight_bounds out ->
+         sep (Bignum out_ptr out) Rout m ->
+         (find k_impl
+          implementing (pred (k (eval out mod M)))
+          with-locals locals and-memory m and-trace tr and-rest R
+          and-functions functions)) ->
+      (let head := v in
+       find (cmd.seq
+               (cmd.call [] square [expr.var x_var; expr.var out_var])
+               k_impl)
+       implementing (pred (dlet head k))
+       with-locals locals and-memory mem and-trace tr and-rest R
+       and-functions functions).
+  Proof.
+    cbv [Placeholder] in *.
+    repeat straightline'.
+    handle_call; [ solve [eauto] .. | ].
+    sepsimpl.
+    repeat match goal with x := _ mod M |- _ =>
+                                subst x end.
+    rewrite Z.pow_2_r in *.
+    match goal with H : _ mod M = ?x mod M
+                    |- context [dlet (?x mod M)] =>
+                    rewrite <-H
+    end.
+    eauto.
+  Qed.
+
+  Lemma compile_scmula24 :
+    forall (locals: Semantics.locals) (mem: Semantics.mem)
+      tr R Rin Rout functions T (pred: T -> _ -> Prop)
+      (x out : bignum) x_ptr x_var out_ptr out_var k k_impl,
+      spec_of_scmula24 functions ->
+      bounded_by loose_bounds x ->
+      (Bignum x_ptr x * Rin)%sep mem ->
+      (Placeholder out_ptr out * Rout)%sep mem ->
+      map.get locals x_var = Some x_ptr ->
+      map.get locals out_var = Some out_ptr ->
+      let v := (a24 * eval x) mod M in
+      (let head := v in
+       forall out m,
+         eval out mod M = head ->
+         bounded_by tight_bounds out ->
+         sep (Bignum out_ptr out) Rout m ->
+         (find k_impl
+          implementing (pred (k (eval out mod M)))
+          with-locals locals and-memory m and-trace tr and-rest R
+          and-functions functions)) ->
+      (let head := v in
+       find (cmd.seq
+               (cmd.call [] scmula24 [expr.var x_var; expr.var out_var])
+               k_impl)
+       implementing (pred (dlet head k))
+       with-locals locals and-memory mem and-trace tr and-rest R
+       and-functions functions).
+  Proof.
+    cbv [Placeholder] in *.
+    repeat straightline'.
+    handle_call; [ solve [eauto] .. | ].
+    sepsimpl.
+    repeat match goal with x := _ mod M |- _ =>
+                                subst x end.
+    match goal with H : _ mod M = ?x mod M
+                    |- context [dlet (?x mod M)] =>
+                    rewrite <-H
+    end.
+    eauto.
+  Qed.
+
+  (* noop indicating that the last argument should store output *)
+  Definition overwrite1 {A B} := @id (A -> B).
+  (* noop indicating that the 2nd-to-last argument should store output *)
+  Definition overwrite2 {A B C} := @id (A -> B -> C).
+
+  Lemma compile_compose_l :
+    forall (locals: Semantics.locals) (mem: Semantics.mem)
+      tr R Rout functions T (pred: T -> _ -> Prop)
+      (op1 op2 : Z -> Z -> Z)
+      x y z out out_ptr out_var k k_impl,
+      (Placeholder out_ptr out * Rout)%sep mem ->
+      map.get locals out_var = Some out_ptr ->
+      let v := ((op2 (op1 x y mod M) z)) mod M in
+      (let head := v in
+       (find k_impl
+        implementing (pred (dlet (op1 x y mod M)
+        (fun xy => dlet ((overwrite2 op2) xy z mod M) k)))
+        with-locals locals and-memory mem and-trace tr and-rest R
+        and-functions functions)) ->
+      (let head := v in
+       find k_impl
+       implementing (pred (dlet head k))
+       with-locals locals and-memory mem and-trace tr and-rest R
+       and-functions functions).
+  Proof.
+    cbv [Placeholder overwrite1 overwrite2] in *.
+    repeat straightline'. auto.
+  Qed.
+
+  Lemma compile_compose_r :
+    forall (locals: Semantics.locals) (mem: Semantics.mem)
+      tr R Rout functions T (pred: T -> _ -> Prop)
+      (op1 op2 : Z -> Z -> Z)
+      x y z out out_ptr out_var k k_impl,
+      (Placeholder out_ptr out * Rout)%sep mem ->
+      map.get locals out_var = Some out_ptr ->
+      let v := ((op2 z (op1 x y mod M))) mod M in
+      (let head := v in
+       (find k_impl
+        implementing (pred (dlet (op1 x y mod M)
+        (fun xy => dlet ((overwrite1 op2) z xy mod M) k)))
+        with-locals locals and-memory mem and-trace tr and-rest R
+        and-functions functions)) ->
+      (let head := v in
+       find k_impl
+       implementing (pred (dlet head k))
+       with-locals locals and-memory mem and-trace tr and-rest R
+       and-functions functions).
+  Proof.
+    cbv [Placeholder overwrite1 overwrite2] in *.
+    repeat straightline'. auto.
+  Qed.
+
+  Lemma compile_overwrite1 :
+    forall (locals: Semantics.locals) (mem: Semantics.mem)
+      tr R Rin functions T (pred: T -> _ -> Prop)
+      (x : Z) (op : Z -> Z -> Z) (y : bignum) y_ptr y_var k k_impl,
+      (Bignum y_ptr y * Rin)%sep mem ->
+      map.get locals y_var = Some y_ptr ->
+      let v := ((overwrite1 op) x (eval y mod M)) mod M in
+      let v' := (op x (eval y mod M)) mod M in
+      (let __ := 0 in (* placeholder *)
+       forall m,
+         sep (Placeholder y_ptr y) Rin m ->
+         (find k_impl
+          implementing (pred (dlet v' k))
+          with-locals locals and-memory m and-trace tr and-rest R
+          and-functions functions)) ->
+      (let head := v in
+       find k_impl
+       implementing (pred (dlet head k))
+       with-locals locals and-memory mem and-trace tr and-rest R
+       and-functions functions).
+  Proof.
+    cbv [Placeholder] in *.
+    repeat straightline'. auto.
+  Qed.
+
+  Lemma compile_overwrite2 :
+    forall (locals: Semantics.locals) (mem: Semantics.mem)
+      tr R Rin functions T (pred: T -> _ -> Prop)
+      (y : Z) (op : Z -> Z -> Z) (x : bignum) x_ptr x_var k k_impl,
+      (Bignum x_ptr x * Rin)%sep mem ->
+      map.get locals x_var = Some x_ptr ->
+      let v := ((overwrite2 op) (eval x mod M) y) mod M in
+      let v' := (op (eval x mod M) y) mod M in
+      (let __ := 0 in (* placeholder *)
+       forall m,
+         sep (Placeholder x_ptr x) Rin m ->
+         (find k_impl
+          implementing (pred (dlet v' k))
+          with-locals locals and-memory m and-trace tr and-rest R
+          and-functions functions)) ->
+      (let head := v in
+       find k_impl
+       implementing (pred (dlet head k))
+       with-locals locals and-memory mem and-trace tr and-rest R
+       and-functions functions).
+  Proof.
+    cbv [Placeholder] in *.
+    repeat straightline'. auto.
+  Qed.
+End Compile.
+
+Module Z.
+  (* helper for Zpow_mod *)
+  Lemma pow_mod_nonneg a b m :
+    0 <= b -> (a ^ b) mod m = ((a mod m) ^ b) mod m.
+  Proof.
+    intros. revert a m.
+    apply natlike_ind with (x:=b); intros;
+      repeat first [ rewrite Z.pow_0_r
+                   | rewrite Z.pow_succ_r by auto
+                   | reflexivity
+                   | solve [auto] ]; [ ].
+    Z.push_mod.
+    match goal with
+      H : context [ (_ ^ _) mod _ = (_ ^ _) mod _ ] |- _ =>
+      rewrite H end.
+    Z.push_pull_mod. reflexivity.
+  Qed.
+
+  (* TODO: upstream to coqutil's Z.pull_mod *)
+  Lemma pow_mod a b m : (a ^ b) mod m = ((a mod m) ^ b) mod m.
+  Proof.
+    destruct (Z_le_dec 0 b); auto using pow_mod_nonneg; [ ].
+    rewrite !Z.pow_neg_r by lia. reflexivity.
+  Qed.
+End Z.
+
+(* TODO: replace with Z.pull_mod once Zpow_mod is upstreamed *)
+Ltac pull_mod :=
+  repeat first [ progress Z.pull_mod
+               | rewrite <-Z.pow_mod ].
+
+Ltac field_compile_step :=
+  Z.push_pull_mod; pull_mod;
+  first [ simple eapply compile_mul
+        | simple eapply compile_add
+        | simple eapply compile_sub
+        | simple eapply compile_square
+        | simple eapply compile_scmula24 ].
+
+Ltac compile_compose_step :=
+  Z.push_mod;
+  first [ simple eapply compile_compose_l
+        | simple eapply compile_compose_r
+        | simple eapply compile_overwrite1
+        | simple eapply compile_overwrite2 ];
+  [ solve [repeat compile_step] .. | intros ].
+
+Ltac compile_custom ::=
+  repeat compile_compose_step;
+  field_compile_step; [ repeat compile_step .. | ];
+  (* if the output we selected was one of the inputs, need to write the
+       Placeholder back into a Bignum for the arguments precondition *)
+  lazymatch goal with
+  | |- sep _ _ _ =>
+    change Placeholder with Bignum in * |- ;
+    solve [repeat compile_step]
+  | _ => idtac
+  end;
+  [ solve [repeat compile_step] .. | intros ].
+
+Ltac overwrite_bignum p := change (Bignum p) with (Placeholder p) in *.
